# baseURI: http://purl.bdrc.io/shapes/core/BaseShapes/
# prefix: BaseShapes

@prefix BaseShapes: <http://purl.bdrc.io/shapes/core/BaseShapes/> .
@prefix adm: <http://purl.bdrc.io/ontology/admin/> .
@prefix bdd: <http://purl.bdrc.io/data/> .
@prefix bdo: <http://purl.bdrc.io/ontology/core/> .
@prefix bdr: <http://purl.bdrc.io/resource/> .
@prefix bds: <http://purl.bdrc.io/ontology/shapes/core/> .
@prefix bf: <http://id.loc.gov/ontologies/bibframe/> .
@prefix cc: <http://creativecommons.org/ns#> .
@prefix dash: <http://datashapes.org/dash#> .
@prefix dcterms: <http://purl.org/dc/terms/> .
@prefix foaf: <http://xmlns.com/foaf/0.1/> .
@prefix iiif2: <http://iiif.io/api/presentation/2#> .
@prefix iiif3: <http://iiif.io/api/presentation/3#> .
@prefix owl: <http://www.w3.org/2002/07/owl#> .
@prefix rdf: <http://www.w3.org/1999/02/22-rdf-syntax-ns#> .
@prefix rdfs: <http://www.w3.org/2000/01/rdf-schema#> .
@prefix sh: <http://www.w3.org/ns/shacl#> .
@prefix skos: <http://www.w3.org/2004/02/skos/core#> .
@prefix swa: <http://topbraid.org/swa#> .
@prefix tbr: <http://purl.bdrc.io/ontology/toberemoved/> .
@prefix tosh: <http://topbraid.org/tosh#> .
@prefix vcard: <http://www.w3.org/2006/vcard/ns#> .
@prefix xml: <http://www.w3.org/XML/1998/namespace> .
@prefix xsd: <http://www.w3.org/2001/XMLSchema#> .

BaseShapes:
  a owl:Ontology ;
  owl:versionInfo "Buda extension to shacl vocabulary" ;
.
bds:RDF 
    a sh:PrefixDeclaration ;
    sh:declare [ 
        sh:prefix "rdf" ;
        sh:namespace "http://www.w3.org/1999/02/22-rdf-syntax-ns#"^^xsd:anyURI ;
    ] ;
.
bds:RDFS
    a sh:PrefixDeclaration ;
    sh:declare [ 
        sh:prefix "rdfs" ;
        sh:namespace "http://www.w3.org/2000/01/rdf-schema#"^^xsd:anyURI ;
    ] ;
.
bds:ADM
    a sh:PrefixDeclaration ;
    sh:declare [ 
        sh:prefix "adm" ;
        sh:namespace "http://purl.bdrc.io/ontology/admin/"^^xsd:anyURI ;
    ] ;
.
bds:BDO
    a sh:PrefixDeclaration ;
    sh:declare [ 
        sh:prefix "bdo" ;
        sh:namespace "http://purl.bdrc.io/ontology/core/"^^xsd:anyURI ;
    ] ;
.
bds:BDR
    a sh:PrefixDeclaration ;
    sh:declare [ 
        sh:prefix "bdr" ;
        sh:namespace "http://purl.bdrc.io/resource/"^^xsd:anyURI ;
    ] ;
.
bds:identifierPrefix
  a owl:DatatypeProperty ;
  rdfs:label "prefix for resource id"@en ;
  rdfs:range xsd:string ;
  skos:definition "prefix to use when generating identifier for a resource"@en ;
.
# TODO: some properties should be displayed conditionally, for instance eventWho on a personEvent only makes sense if the type of personEvent is a marriage or divorce
bds:displayPriority
  a owl:DatatypeProperty ;
  rdfs:label "display priority"@en ;
  rdfs:range xsd:integer ;
  rdfs:domain sh:PropertyShape ;
  skos:definition "indicates if a property should be displayed or hidden, using a number between 0 and 2 where 0 means the property should always be displayed, 1 means the property can be hidden behind a see more button if necessary, 2 means the property should be hidden unless there's an associated value, and 3 means that the property should always be hidden (use for inferred fields for instance)."@en ;
.
bds:classIn
  a owl:DatatypeProperty ;
  rdfs:label "expected object type"@en ;
  rdfs:domain rdfs:Resource ;
  skos:definition "this is similar to sh:class except that the constraint is that the type must be any of the listed types instead of the conjuction of all listed types. The object should be a rdf:list."@en ;
.
bds:nodeShapeType
  a owl:ObjectProperty ;
  rdfs:label "node shape type"@en ;
  rdfs:domain sh:NodeShape ;
  rdfs:range bds:ShapeType ;
  skos:definition "type of a node shape to discriminate among fact shapes, internal shapes, and so on"@en ;
.
bds:propertyShapeType
  a owl:ObjectProperty ;
  rdfs:label "node shape type"@en ;
  rdfs:domain sh:PropertyShape ;
  rdfs:range bds:ShapeType ;
  skos:definition "type of a node shape to discriminate among fact shapes, internal shapes, and so on"@en ;
.
bds:allowMarkDown
  a owl:DatatypeProperty ;
  rdfs:label "node shape type"@en ;
  rdfs:domain sh:PropertyShape ;
  rdfs:range xsd:boolean ;
  skos:definition "the object of the property can be in markdown"@en ;
.
bds:ShapeType
  a owl:Class ;
.
bds:independentIdentifiers
  a owl:DatatypeProperty ;
  rdfs:label "independent identifiers"@en ;
  rdfs:domain sh:NodeShape ;
  rdfs:range xsd:boolean ;
  skos:definition "the identifiers for the resource are independent from its parent resource"@en ;
.
bds:sortOnProperty
  a owl:ObjectProperty ;
  rdfs:label "sort on property"@en ;
  rdfs:domain sh:PropertyShape ;
  skos:definition "sort the objects of the property shape by one of their property. This is for display purpose only and has no effect on the data."@en ;
.
bds:ExternalShape
  a bds:ShapeType ;
  rdfs:label "node shape refers to resource external to focus node graph"@en ;
  skos:definition "this shape indicates external resource that is not contained in the focus node graph"@en ;
.
bds:FacetShape
  a bds:ShapeType ;
  rdfs:label "node shape is a facet"@en ;
  skos:definition "this shape applies to a resource contained in the graph of root Resource that is a facet of the containing resource"@en ;
.
bds:IgnoreShape
  a bds:ShapeType ;
  rdfs:label "node shape is ignored for editing"@en ;
  skos:definition "this shape indicates internal resource that is not editable"@en ;
.
bds:InternalShape
  a bds:ShapeType ;
  rdfs:label "node shape is internal"@en ;
  skos:definition "this shape applies to internal resources such as Volumes in an Imagegroup"@en ;
.
bds:increment
  a owl:DatatypeProperty ;
  rdfs:label "increment by"@en ;
  rdfs:domain sh:PropertyShape ;
  rdfs:range xsd:integer ;
  skos:definition "an amount to increment the value of the sh:path property by"@en ;
.
bds:sortBy
  a owl:DatatypeProperty ;
  rdfs:label "sort rank"@en ;
  rdfs:domain sh:PropertyShape ;
  skos:definition "the property (value of sh:path, not shacl property) used to sort the objects of this property"@en ;
.
bds:sortRank
  a owl:DatatypeProperty ;
  rdfs:label "sort rank"@en ;
  rdfs:domain sh:PropertyShape ;
  rdfs:range xsd:integer ;
  skos:definition "values of the sh:path property are used to sort results before higher ranked properties."@en ;
.
bds:sortDirection
  a owl:ObjecttypeProperty ;
  rdfs:label "sort direction"@en ;
  rdfs:domain sh:PropertyShape ;
  rdfs:range bds:SortDirection ;
  skos:definition "values of the sh:path property are sorted in the specified direction."@en ;
.
bds:SortDirection
  a owl:Class ;
.
bds:SortAscending
  a bds:SortDirection ;
  rdfs:label "sort ascending"@en ;
  skos:definition "items should be sorted in ascending order"@en ;
.
bds:SortDescending
  a bds:SortDirection ;
  rdfs:label "sort descending"@en ;
  skos:definition "items should be sorted in descending order"@en ;
.
bds:topShapeGraph
  a owl:ObjectProperty ;
  rdfs:domain bdo:Entity ;
  rdfs:range xsd:anyURI ;
.
bds:uiShapeGraph
  a owl:ObjectProperty ;
  rdfs:domain bdo:Entity ;
  rdfs:range xsd:anyURI ;
.
bds:uiShapeGraph
  a owl:ObjectProperty ;
  rdfs:domain bdo:Entity ;
  rdfs:range xsd:anyURI ;
.
bds:readOnly
  a owl:DatatypeProperty ;
  rdfs:label "read only"@en ;
  rdfs:domain sh:PropertyShape ;
  rdfs:range xsd:boolean ;
  skos:definition "true indicates that the editor should not allow the user to change the property"@en ;
.
bds:defaultValue
  a owl:DatatypeProperty ;
  rdfs:label "editor default value"@en ;
  rdfs:domain sh:PropertyShape ;
  skos:definition "indicates the default value that the editor should display when there is no value"@en ;
.
bds:defaultLanguage
  a owl:DatatypeProperty ;
  rdfs:label "default language"@en ;
  rdfs:domain sh:PropertyShape ;
  rdfs:range xsd:string ;
  skos:definition "indicates the default language that the editor should display for the values of a certain property"@en ;
.
# blank nodes make it so that if the same file is imported twice, things will go wrong...
# what a wonderful format RDF is...
bds:DateTimeOrDateOrgYear
  a rdf:List ;
  rdf:first [
      sh:datatype xsd:dateTime ;
    ] ;
  rdf:rest (
      [
        sh:datatype xsd:date ;
      ]
      [
        sh:datatype xsd:gYear ;
      ]
    ) ;
  rdfs:comment "An rdf:List that can be used in property constraints as value for sh:or to indicate that all values of a property must be either xsd:gYear, xsd:date or xsd:dateTime." ;
  rdfs:label "Date or date time or year" ;
.
# defining the path to use in the list path pattern (https://www.topquadrant.com/constraints-on-rdflists-using-shacl/)
bds:listPathZeroOrMore sh:zeroOrMorePath rdf:rest .
bds:listPath rdf:first bds:listPathZeroOrMore ;
             rdf:rest rdf:first .

bds:specialPattern
  a owl:ObjectProperty ;
  rdfs:domain sh:PropertyShape ;
  rdfs:range bds:SpecialPattern ;
  skos:prefLabel "special pattern"@en ;
.

bds:SpecialPattern
  a owl:Class ;
.
bds:PatternEDTF
  a bds:SpecialPattern ;
  skos:prefLabel "EDTF pattern"@en ;
  skos:description "Extended Date/Time Format (EDTF) has been designed by the Library of Congress and integrated into ISO8601-2019"@en ;
  rdfs:seeAlso <https://www.loc.gov/standards/datetime/> ;
.
bds:PatternISBN
  a bds:SpecialPattern ;
  skos:prefLabel "ISBN pattern"@en ;
.