# baseURI: http://purl.bdrc.io/shapes/core/BaseShapes/
# imports: http://datashapes.org/dash
# imports: http://purl.bdrc.io/ontology/core/
# prefix: BaseShapes

@prefix BaseShapes: <http://purl.bdrc.io/shapes/core/BaseShapes/> .
@prefix adm: <http://purl.bdrc.io/ontology/admin/> .
@prefix bdd: <http://purl.bdrc.io/data/> .
@prefix bdo: <http://purl.bdrc.io/ontology/core/> .
@prefix bdr: <http://purl.bdrc.io/resource/> .
@prefix bds: <http://purl.bdrc.io/ontology/shapes/core/> .
@prefix bf: <http://id.loc.gov/ontologies/bibframe/> .
@prefix cc: <http://creativecommons.org/ns#> .
@prefix dash: <http://datashapes.org/dash#> .
@prefix dcterms: <http://purl.org/dc/terms/> .
@prefix foaf: <http://xmlns.com/foaf/0.1/> .
@prefix iiif2: <http://iiif.io/api/presentation/2#> .
@prefix iiif3: <http://iiif.io/api/presentation/3#> .
@prefix owl: <http://www.w3.org/2002/07/owl#> .
@prefix rdf: <http://www.w3.org/1999/02/22-rdf-syntax-ns#> .
@prefix rdfs: <http://www.w3.org/2000/01/rdf-schema#> .
@prefix sh: <http://www.w3.org/ns/shacl#> .
@prefix skos: <http://www.w3.org/2004/02/skos/core#> .
@prefix swa: <http://topbraid.org/swa#> .
@prefix tbr: <http://purl.bdrc.io/ontology/toberemoved/> .
@prefix tosh: <http://topbraid.org/tosh#> .
@prefix vcard: <http://www.w3.org/2006/vcard/ns#> .
@prefix xml: <http://www.w3.org/XML/1998/namespace> .
@prefix xsd: <http://www.w3.org/2001/XMLSchema#> .

BaseShapes:
  a owl:Ontology ;
  owl:imports <http://datashapes.org/dash> ;
  owl:versionInfo "Buda extension to shacl vocabulary" ;
.
bds:identifierPrefix
  a owl:DatatypeProperty ;
  rdfs:label "prefix for resource id"@en ;
  rdfs:domain rdfs:Resource ;
  rdfs:range xsd:string ;
  skos:definition "prefix to use when generating identifier for a resource"@en ;
.
bds:nodeShapeType
  a owl:ObjectProperty ;
  rdfs:label "node shape type"@en ;
  rdfs:domain sh:NodeShape ;
  rdfs:range bds:ShapeType ;
  skos:definition "type of a node shape to discriminate among fact shapes, internal shapes, and so on"@en ;
.
bds:propertyShapeType
  a owl:ObjectProperty ;
  rdfs:label "node shape type"@en ;
  rdfs:domain sh:PropertyShape ;
  rdfs:range bds:ShapeType ;
  skos:definition "type of a node shape to discriminate among fact shapes, internal shapes, and so on"@en ;
.
bds:ShapeType
  a owl:Class ;
.
bds:FacetShape
  a bds:ShapeType ;
  rdfs:label "node shape is a facet"@en ;
  skos:definition "this shape applies to a resource contained in the graph of root Resource that is a facet of the containing resource"@en ;
.
bds:IgnoreShape
  a bds:ShapeType ;
  rdfs:label "node shape is ignored for editing"@en ;
  skos:definition "this shape indicates internal resource that is not editable"@en ;
.
bds:InternalShape
  a bds:ShapeType ;
  rdfs:label "node shape is internal"@en ;
  skos:definition "this shape applies to internal resources such as Volumes in an Imagegroup"@en ;
.
